Imp: Some copy-paste from the book, no solutions here.

Imp/Imp.v
@@ -309,6 +309,8 @@ Proof.
             try apply IHa1; try apply IHa2; reflexivity.
 Qed.
 
+End AExp.
+
 Module aevalR_division.
 
 Inductive aexp : Type :=
@@ -497,3 +499,191 @@ Proof.
         SCase "x2 <> x3".
             reflexivity.
 Qed.
+
+Inductive aexp : Type :=
+| ANum : nat -> aexp
+| AId : id -> aexp
+| APlus : aexp -> aexp -> aexp
+| AMinus : aexp -> aexp -> aexp
+| AMult : aexp -> aexp ->aexp.
+
+Tactic Notation "aexp_cases" tactic(first) ident(c) :=
+    first;
+    [ Case_aux c "ANum" | Case_aux c "AId" | Case_aux c "APlus"
+    | Case_aux c "AMinus" | Case_aux c "AMult" ].
+
+Definition X : id := Id 0.
+Definition Y : id := Id 1.
+Definition Z : id := Id 2.
+
+Inductive bexp : Type :=
+| BTrue : bexp
+| BFalse : bexp
+| BEq : aexp -> aexp -> bexp
+| BLe : aexp -> aexp -> bexp
+| BNot : bexp -> bexp
+| BAnd : bexp -> bexp -> bexp.
+
+Tactic Notation "bexp_cases" tactic(first) ident(c) :=
+    first;
+    [ Case_aux c "BTrue" | Case_aux c "BFalse" | Case_aux c "BEq"
+    | Case_aux c "BLe" | Case_aux c "BNot" | Case_aux c "BAnd" ].
+
+Fixpoint aeval (st : state) (a : aexp) : nat :=
+    match a with
+    | ANum n => n
+    | AId x => st x
+    | APlus a1 a2 => (aeval st a1) + (aeval st a2)
+    | AMinus a1 a2 => (aeval st a1) - (aeval st a2)
+    | AMult a1 a2 => (aeval st a1) * (aeval st a2)
+    end.
+
+Fixpoint beval (st : state) (b : bexp) : bool :=
+    match b with
+    | BTrue => true
+    | BFalse => false
+    | BEq a1 a2 => beq_nat (aeval st a1) (aeval st a2)
+    | BLe a1 a2 => ble_nat (aeval st a1) (aeval st a2)
+    | BNot b1 => negb (beval st b1)
+    | BAnd b1 b2 => andb (beval st b1) (beval st b2)
+    end.
+
+Example aexp1 :
+    aeval (update empty_state X 5)
+          (APlus (ANum 3) (AMult (AId X) (ANum 2)))
+    = 13.
+Proof. reflexivity. Qed.
+
+Example bexp2 :
+    beval (update empty_state X 5)
+          (BAnd BTrue (BNot (BLe (AId X) (ANum 4))))
+    = true.
+Proof. reflexivity. Qed.
+
+Inductive com : Type :=
+| CSkip : com
+| CAss : id -> aexp -> com
+| CSeq : com -> com -> com
+| CIf : bexp -> com -> com -> com
+| CWhile : bexp -> com -> com.
+
+Tactic Notation "com_cases" tactic(first) ident(c) :=
+    first;
+    [ Case_aux c "SKIP" | Case_aux c "::=" | Case_aux c ";;"
+    | Case_aux c "IFB" | Case_aux c "WHILE" ].
+
+Notation "'SKIP'" :=
+    CSkip.
+Notation "x '::=' a" :=
+    (CAss x a) (at level 60).
+Notation "c1 ;; c2" :=
+    (CSeq c1 c2) (at level 80, right associativity).
+Notation "'WHILE' b 'DO' c 'END'" :=
+    (CWhile b c) (at level 80, right associativity).
+Notation "'IFB' c1 'THEN' c2 'ELSE' c3 'FI'" :=
+    (CIf c1 c2 c3) (at level 80, right associativity).
+
+Definition fact_in_coq : com :=
+    Z ::= AId X;;
+    Y ::= ANum 1;;
+    WHILE BNot (BEq (AId Z) (ANum 0)) DO
+        Y ::= AMult (AId Y) (AId Z);;
+        Z ::= AMinus (AId Z) (ANum 1)
+    END.
+
+Definition plus2 : com :=
+    X ::= (APlus (AId X) (ANum 2)).
+
+Definition XtimesYinZ : com :=
+    Z ::= (AMult (AId X) (AId Y)).
+
+Definition substract_slowly_body : com :=
+    Z ::= AMinus (AId Z) (ANum 1) ;;
+    X ::= AMinus (AId X) (ANum 1).
+
+Definition substract_slowly : com :=
+    WHILE BNot (BEq (AId X) (ANum 0)) DO
+        substract_slowly_body
+    END.
+
+Definition substract_3_from_5_slowly : com :=
+    X ::= ANum 3;;
+    Z ::= ANum 5;;
+    substract_slowly.
+
+Definition loop : com :=
+    WHILE BTrue DO
+        SKIP
+    END.
+
+
+Fixpoint ceval_fun_no_while (st : state) (c : com) : state :=
+    match c with
+    | SKIP => st
+    | x ::= a1 =>
+        update st x (aeval st a1)
+    | c1 ;; c2 =>
+        let st' := ceval_fun_no_while st c1 in
+        ceval_fun_no_while st' c2
+    | IFB b THEN c1 ELSE c2 FI =>
+        if (beval st b)
+            then ceval_fun_no_while st c1
+            else ceval_fun_no_while st c2
+    | WHILE b DO c END =>
+        st
+    end.
+
+Reserved Notation "c1 '/' st '||' st'" (at level 40, st at level 39).
+
+Inductive ceval : com -> state -> state -> Prop :=
+  | E_Skip : forall st,
+      SKIP / st || st
+  | E_Ass : forall st a1 n x,
+      aeval st a1 = n ->
+      (x ::= a1) / st || (update st x n)
+  | E_Seq : forall c1 c2 st st' st'',
+      c1 / st || st' ->
+      c2 / st' || st'' ->
+      (c1 ;; c2) / st || st''
+  | E_IfTrue : forall st st' b c1 c2,
+      beval st b = true ->
+      c1 / st || st' ->
+      (IFB b THEN c1 ELSE c2 FI) / st || st'
+  | E_IfFalse : forall st st' b c1 c2,
+      beval st b = false ->
+      c2 / st || st' ->
+      (IFB b THEN c1 ELSE c2 FI) / st || st'
+  | E_WhileEnd : forall b st c,
+      beval st b = false ->
+      (WHILE b DO c END) / st || st
+  | E_WhileLoop : forall st st' st'' b c,
+      beval st b = true ->
+      c / st || st' ->
+      (WHILE b DO c END) / st' || st'' ->
+      (WHILE b DO c END) / st || st''
+
+  where "c1 '/' st '||' st'" := (ceval c1 st st').
+
+Tactic Notation "ceval_cases" tactic(first) ident(c) :=
+  first;
+  [ Case_aux c "E_Skip" | Case_aux c "E_Ass" | Case_aux c "E_Seq"
+  | Case_aux c "E_IfTrue" | Case_aux c "E_IfFalse"
+  | Case_aux c "E_WhileEnd" | Case_aux c "E_WhileLoop" ].
+
+Example ceval_example:
+    (X ::= ANum 2;;
+     IFB BLe (AId X) (ANum 1)
+        THEN Y ::= ANum 3
+        ELSE Z ::= ANum 4
+     FI)
+     / empty_state
+     || (update (update empty_state X 2) Z 4).
+Proof.
+  (* We must supply the intermediate state *)
+  apply E_Seq with (update empty_state X 2).
+  Case "assignment command".
+    apply E_Ass. reflexivity.
+  Case "if command".
+    apply E_IfFalse.
+      reflexivity.
+      apply E_Ass. reflexivity. Qed.
